Tweak

demo/mutrec/MutrecABspec.v
@@ -5,8 +5,10 @@ Require Import sflib.
 Require Import SmallstepC.
 Require Export Simulation.
 Require Import Skeleton Mod ModSem.
-Require Import AsmC.
-Require Import MutrecHeader MutrecB.
+Require Import CtypesC CtypingC.
+Require Import ClightC.
+Require Import MutrecHeader.
+Require Import MutrecA.
 
 Set Implicit Arguments.
 
@@ -15,9 +17,9 @@ Local Obligation Tactic := ii; ss; des; inv_all_once; ss; clarify.
 Section MODSEM.
 
   Variable skenv_link: SkEnv.t.
-  Variable p: unit.
-  Let skenv: SkEnv.t := skenv_link.(SkEnv.project) prog.(Sk.of_program fn_sig).
-  Let ge: genv := skenv.(SkEnv.revive) prog.
+  Variable p: program.
+  Let skenv: SkEnv.t := skenv_link.(SkEnv.project) p.(CSk.of_program signature_of_function).
+  Let ge: genv := Build_genv (skenv.(SkEnv.revive) p) p.(prog_comp_env).
 
   Inductive state: Type :=
   | Callstate
@@ -37,39 +39,19 @@ Section MODSEM.
 
   Inductive initial_frame (args: Args.t): state -> Prop :=
   | initial_frame1_intro
-      i m
-      (FINDF: Genv.find_funct ge args.(Args.fptr) = Some (Internal func_g))
+      i m func_fg
+      (FINDF: Genv.find_funct ge args.(Args.fptr) = Some (Internal func_fg))
       (VS: args.(Args.vs) = [Vint i])
       (M: args.(Args.m) = m)
     :
       initial_frame args (Callstate i m)
   .
 
-  Inductive at_external: state -> Args.t -> Prop :=
-  | at_external_intro
-      f_fptr i m
-      (FINDG: Genv.find_symbol ge f_id = Some f_fptr)
-      (NZERO: i.(Int.intval) <> 0%Z)
-    :
-      at_external (Callstate i m) (Args.mk (Vptr f_fptr Ptrofs.zero) [Vint (Int.sub i (Int.repr 1))] m)
-  .
-
-  Inductive after_external: state -> Retv.t -> state -> Prop :=
-  | after_external_intro
-      i m retv
-      i_after
-      (INT: retv.(Retv.v) = Vint i_after)
-      (SUM: i_after = sum (Int.sub i Int.one))
-    :
-      after_external (Callstate i m) retv (Returnstate (sum i) retv.(Retv.m))
-  .
-
   Inductive step (se: Senv.t) (ge: genv): state -> trace -> state -> Prop :=
   | step_zero
       i m
-      (ZERO: i.(Int.intval) = 0%Z)
     :
-      step se ge (Callstate i m) E0 (Returnstate i m)
+      step se ge (Callstate i m) E0 (Returnstate (sum i) m)
   .
 
   Inductive final_frame: state -> Retv.t -> Prop :=
@@ -82,10 +64,10 @@ Section MODSEM.
   Program Definition modsem: ModSem.t :=
     {|
       ModSem.step := step;
-      ModSem.at_external := at_external;
+      ModSem.at_external := bot2;
       ModSem.initial_frame := initial_frame;
       ModSem.final_frame := final_frame;
-      ModSem.after_external := after_external;
+      ModSem.after_external := bot3;
       ModSem.globalenv := ge;
       ModSem.skenv := skenv;
       ModSem.skenv_link := skenv_link; 
@@ -94,5 +76,5 @@ Section MODSEM.
 
 End MODSEM.
 
-Program Definition module: Mod.t :=
-  {| Mod.data := tt; Mod.get_sk := fun _ => Sk.of_program fn_sig prog; Mod.get_modsem := modsem; |}.
+Program Definition module (p: program): Mod.t :=
+  {| Mod.data := p; Mod.get_sk := CSk.of_program signature_of_function; Mod.get_modsem := modsem; |}.
